specs/L2InteropHandler/L2InteropHandler/Common/if_935801784454999646_user.lean
@@ -12,12 +12,13 @@ section
 
 open Clear EVMState Ast Expr Stmt FunctionDefinition State Interpreter ExecLemmas OutOfFuelLemmas Abstraction YulNotation PrimOps ReasoningPrinciple Utilities L2InteropHandler.Common 
 
-def A_if_935801784454999646 (s₀ s₉ : State) : Prop := sorry
+def A_if_935801784454999646 (s₀ s₉ : State) : Prop := if_935801784454999646_concrete_of_code.1 s₀ s₉
 
 lemma if_935801784454999646_abs_of_concrete {s₀ s₉ : State} :
   Spec if_935801784454999646_concrete_of_code s₀ s₉ →
   Spec A_if_935801784454999646 s₀ s₉ := by
-  sorry
+  intro h
+  simpa [A_if_935801784454999646] using h
 
 end
 
