specs/L2InteropHandler/L2InteropHandler/Common/switch_8523945878344766818_user.lean
@@ -10,12 +10,13 @@ section
 
 open Clear EVMState Ast Expr Stmt FunctionDefinition State Interpreter ExecLemmas OutOfFuelLemmas Abstraction YulNotation PrimOps ReasoningPrinciple Utilities 
 
-def A_switch_8523945878344766818 (s₀ s₉ : State) : Prop := sorry
+def A_switch_8523945878344766818 (s₀ s₉ : State) : Prop := switch_8523945878344766818_concrete_of_code.1 s₀ s₉
 
 lemma switch_8523945878344766818_abs_of_concrete {s₀ s₉ : State} :
   Spec switch_8523945878344766818_concrete_of_code s₀ s₉ →
   Spec A_switch_8523945878344766818 s₀ s₉ := by
-  sorry
+  intro h
+  simpa [A_switch_8523945878344766818] using h
 
 end
 
