specs/L2InteropHandler/L2InteropHandler/abi_decode_bytest_struct_MessageInclusionProof_21940_user.lean
@@ -40,13 +40,13 @@ section
 
 open Clear EVMState Ast Expr Stmt FunctionDefinition State Interpreter ExecLemmas OutOfFuelLemmas Abstraction YulNotation PrimOps ReasoningPrinciple Utilities L2InteropHandler.Common generated.L2InteropHandler L2InteropHandler
 
-def A_abi_decode_bytest_struct_MessageInclusionProof_21940 (value0 value1 : Identifier) (dataEnd : Literal) (s₀ s₉ : State) : Prop := sorry
+def A_abi_decode_bytest_struct_MessageInclusionProof_21940 (value0 value1 : Identifier) (dataEnd : Literal) (s₀ s₉ : State) : Prop := abi_decode_bytest_struct_MessageInclusionProof_21940_concrete_of_code.1 value0 value1 dataEnd s₀ s₉
 
 lemma abi_decode_bytest_struct_MessageInclusionProof_21940_abs_of_concrete {s₀ s₉ : State} {value0 value1 dataEnd} :
   Spec (abi_decode_bytest_struct_MessageInclusionProof_21940_concrete_of_code.1 value0 value1 dataEnd) s₀ s₉ →
   Spec (A_abi_decode_bytest_struct_MessageInclusionProof_21940 value0 value1 dataEnd) s₀ s₉ := by
-  unfold abi_decode_bytest_struct_MessageInclusionProof_21940_concrete_of_code A_abi_decode_bytest_struct_MessageInclusionProof_21940
-  sorry
+  intro h
+  simpa [A_abi_decode_bytest_struct_MessageInclusionProof_21940] using h
 
 end
 
