specs/L2InteropHandler/L2InteropHandler/abi_encode_bytes32_bytes_calldata_bytes_user.lean
@@ -14,13 +14,13 @@ section
 
 open Clear EVMState Ast Expr Stmt FunctionDefinition State Interpreter ExecLemmas OutOfFuelLemmas Abstraction YulNotation PrimOps ReasoningPrinciple Utilities L2InteropHandler.Common generated.L2InteropHandler L2InteropHandler
 
-def A_abi_encode_bytes32_bytes_calldata_bytes (tail : Identifier) (headStart value0 value1 value2 value3 : Literal) (s₀ s₉ : State) : Prop := sorry
+def A_abi_encode_bytes32_bytes_calldata_bytes (tail : Identifier) (headStart value0 value1 value2 value3 : Literal) (s₀ s₉ : State) : Prop := abi_encode_bytes32_bytes_calldata_bytes_concrete_of_code.1 tail headStart value0 value1 value2 value3 s₀ s₉
 
 lemma abi_encode_bytes32_bytes_calldata_bytes_abs_of_concrete {s₀ s₉ : State} {tail headStart value0 value1 value2 value3} :
   Spec (abi_encode_bytes32_bytes_calldata_bytes_concrete_of_code.1 tail headStart value0 value1 value2 value3) s₀ s₉ →
   Spec (A_abi_encode_bytes32_bytes_calldata_bytes tail headStart value0 value1 value2 value3) s₀ s₉ := by
-  unfold abi_encode_bytes32_bytes_calldata_bytes_concrete_of_code A_abi_encode_bytes32_bytes_calldata_bytes
-  sorry
+  intro h
+  simpa [A_abi_encode_bytes32_bytes_calldata_bytes] using h
 
 end
 
