specs/L2InteropHandler/L2InteropHandler/abi_encode_enum_CallStatus_user.lean
@@ -11,13 +11,13 @@ section
 
 open Clear EVMState Ast Expr Stmt FunctionDefinition State Interpreter ExecLemmas OutOfFuelLemmas Abstraction YulNotation PrimOps ReasoningPrinciple Utilities L2InteropHandler.Common 
 
-def A_abi_encode_enum_CallStatus  (value pos : Literal) (s₀ s₉ : State) : Prop := sorry
+def A_abi_encode_enum_CallStatus  (value pos : Literal) (s₀ s₉ : State) : Prop := abi_encode_enum_CallStatus_concrete_of_code.1 value pos s₀ s₉
 
 lemma abi_encode_enum_CallStatus_abs_of_concrete {s₀ s₉ : State} { value pos} :
   Spec (abi_encode_enum_CallStatus_concrete_of_code.1  value pos) s₀ s₉ →
   Spec (A_abi_encode_enum_CallStatus  value pos) s₀ s₉ := by
-  unfold abi_encode_enum_CallStatus_concrete_of_code A_abi_encode_enum_CallStatus
-  sorry
+  intro h
+  simpa [A_abi_encode_enum_CallStatus] using h
 
 end
 
