specs/L2InteropHandler/L2InteropHandler/finalize_allocation_21964_user.lean
@@ -11,13 +11,13 @@ section
 
 open Clear EVMState Ast Expr Stmt FunctionDefinition State Interpreter ExecLemmas OutOfFuelLemmas Abstraction YulNotation PrimOps ReasoningPrinciple Utilities L2InteropHandler.Common 
 
-def A_finalize_allocation_21964  (memPtr : Literal) (s₀ s₉ : State) : Prop := sorry
+def A_finalize_allocation_21964  (memPtr : Literal) (s₀ s₉ : State) : Prop := finalize_allocation_21964_concrete_of_code.1 memPtr s₀ s₉
 
 lemma finalize_allocation_21964_abs_of_concrete {s₀ s₉ : State} { memPtr} :
   Spec (finalize_allocation_21964_concrete_of_code.1  memPtr) s₀ s₉ →
   Spec (A_finalize_allocation_21964  memPtr) s₀ s₉ := by
-  unfold finalize_allocation_21964_concrete_of_code A_finalize_allocation_21964
-  sorry
+  intro h
+  simpa [A_finalize_allocation_21964] using h
 
 end
 
