specs/L2InteropHandler/L2InteropHandler/fun_getBundleData_user.lean
@@ -52,13 +52,13 @@ section
 
 open Clear EVMState Ast Expr Stmt FunctionDefinition State Interpreter ExecLemmas OutOfFuelLemmas Abstraction YulNotation PrimOps ReasoningPrinciple Utilities L2InteropHandler.Common generated.L2InteropHandler L2InteropHandler
 
-def A_fun_getBundleData (var_interopBundle_2782_mpos var_bundleHash var_currentStatus : Identifier) (var_bundle_mpos : Literal) (s₀ s₉ : State) : Prop := sorry
+def A_fun_getBundleData (var_interopBundle_2782_mpos var_bundleHash var_currentStatus : Identifier) (var_bundle_mpos : Literal) (s₀ s₉ : State) : Prop := fun_getBundleData_concrete_of_code.1 var_interopBundle_2782_mpos var_bundleHash var_currentStatus var_bundle_mpos s₀ s₉
 
 lemma fun_getBundleData_abs_of_concrete {s₀ s₉ : State} {var_interopBundle_2782_mpos var_bundleHash var_currentStatus var_bundle_mpos} :
   Spec (fun_getBundleData_concrete_of_code.1 var_interopBundle_2782_mpos var_bundleHash var_currentStatus var_bundle_mpos) s₀ s₉ →
   Spec (A_fun_getBundleData var_interopBundle_2782_mpos var_bundleHash var_currentStatus var_bundle_mpos) s₀ s₉ := by
-  unfold fun_getBundleData_concrete_of_code A_fun_getBundleData
-  sorry
+  intro h
+  simpa [A_fun_getBundleData] using h
 
 end
 
