specs/L2InteropHandler/L2InteropHandler/fun_parseEvmV1_user.lean
@@ -17,13 +17,13 @@ section
 
 open Clear EVMState Ast Expr Stmt FunctionDefinition State Interpreter ExecLemmas OutOfFuelLemmas Abstraction YulNotation PrimOps ReasoningPrinciple Utilities L2InteropHandler.Common generated.L2InteropHandler L2InteropHandler
 
-def A_fun_parseEvmV1 (var_chainId var_addr : Identifier) (var_self_3868_mpos : Literal) (s₀ s₉ : State) : Prop := sorry
+def A_fun_parseEvmV1 (var_chainId var_addr : Identifier) (var_self_3868_mpos : Literal) (s₀ s₉ : State) : Prop := fun_parseEvmV1_concrete_of_code.1 var_chainId var_addr var_self_3868_mpos s₀ s₉
 
 lemma fun_parseEvmV1_abs_of_concrete {s₀ s₉ : State} {var_chainId var_addr var_self_3868_mpos} :
   Spec (fun_parseEvmV1_concrete_of_code.1 var_chainId var_addr var_self_3868_mpos) s₀ s₉ →
   Spec (A_fun_parseEvmV1 var_chainId var_addr var_self_3868_mpos) s₀ s₉ := by
-  unfold fun_parseEvmV1_concrete_of_code A_fun_parseEvmV1
-  sorry
+  intro h
+  simpa [A_fun_parseEvmV1] using h
 
 end
 
