specs/L2InteropHandler/L2InteropHandler/require_helper_error_ExecutingNotAllowed_bytes32_bytes_bytes_user.lean
@@ -12,13 +12,13 @@ section
 
 open Clear EVMState Ast Expr Stmt FunctionDefinition State Interpreter ExecLemmas OutOfFuelLemmas Abstraction YulNotation PrimOps ReasoningPrinciple Utilities L2InteropHandler.Common generated.L2InteropHandler L2InteropHandler
 
-def A_require_helper_error_ExecutingNotAllowed_bytes32_bytes_bytes  (condition expr expr_2409_mpos expr_2412_mpos : Literal) (s₀ s₉ : State) : Prop := sorry
+def A_require_helper_error_ExecutingNotAllowed_bytes32_bytes_bytes  (condition expr expr_2409_mpos expr_2412_mpos : Literal) (s₀ s₉ : State) : Prop := require_helper_error_ExecutingNotAllowed_bytes32_bytes_bytes_concrete_of_code.1 condition expr expr_2409_mpos expr_2412_mpos s₀ s₉
 
 lemma require_helper_error_ExecutingNotAllowed_bytes32_bytes_bytes_abs_of_concrete {s₀ s₉ : State} { condition expr expr_2409_mpos expr_2412_mpos} :
   Spec (require_helper_error_ExecutingNotAllowed_bytes32_bytes_bytes_concrete_of_code.1  condition expr expr_2409_mpos expr_2412_mpos) s₀ s₉ →
   Spec (A_require_helper_error_ExecutingNotAllowed_bytes32_bytes_bytes  condition expr expr_2409_mpos expr_2412_mpos) s₀ s₉ := by
-  unfold require_helper_error_ExecutingNotAllowed_bytes32_bytes_bytes_concrete_of_code A_require_helper_error_ExecutingNotAllowed_bytes32_bytes_bytes
-  sorry
+  intro h
+  simpa [A_require_helper_error_ExecutingNotAllowed_bytes32_bytes_bytes] using h
 
 end
 
